fairneris/examples/retransmit_model.v
@@ -1,7 +1,7 @@
 From trillium.prelude Require Export finitary quantifiers sigma classical_instances.
 From Paco Require Import paco1 paco2 pacotac.
-From fairneris Require Export trace_utils fairness.
-From fairneris.aneris_lang Require Import ast network lang.
+From fairneris Require Export trace_utils fairness env_model.
+From fairneris.aneris_lang Require Import ast network lang aneris_lang.
 From fairneris Require Export trace_utils ltl_lite.
 
 Import derived_laws_later.bi.
@@ -62,9 +62,9 @@ Inductive retransmit_trans :
 | A_Send st :
   retransmit_trans st (Arole, Some (Send mAB)) st
 | B_RecvFail :
-  retransmit_trans Start (Brole, Some (Recv None)) Start
+  retransmit_trans Start (Brole, Some (Recv saB None)) Start
 | B_RecvSucc msg :
-  retransmit_trans Start (Brole, Some (Recv (Some msg))) Received
+  retransmit_trans Start (Brole, Some (Recv saB (Some msg))) Received
 .
 Notation mtrace := (trace retransmit_state (retransmit_role * option aneris_action)).
 
@@ -86,30 +86,30 @@ Instance send_filter_decision msg st l : Decision (send_filter msg st l).
 Proof. apply make_decision. Qed.
 
 Definition recv_filter msg : retransmit_state → retransmit_label → Prop :=
-  λ _ l, snd l = Some $ Recv (Some msg).
+  λ _ l, snd l = Some $ Recv (m_destination msg) (Some msg).
 Instance recv_filter_decision msg st l : Decision (recv_filter msg st l).
 Proof. apply make_decision. Qed.
 
-Definition any_recv_filter : retransmit_state → retransmit_label → Prop :=
-  λ _ l, exists rcv, snd l = Some $ Recv rcv.
-Instance any_recv_filter_decision st l : Decision (any_recv_filter st l).
+Definition any_recv_filter sa : retransmit_state → retransmit_label → Prop :=
+  λ _ l, exists rcv, snd l = Some $ Recv sa rcv.
+Instance any_recv_filter_decision st l sa : Decision (any_recv_filter sa st l).
 Proof. apply make_decision. Qed.
 
 Definition retransmit_fair_network_delivery msg : mtrace → Prop :=
-  □ (□◊!↓send_filter msg → □◊!↓ any_recv_filter → ◊!↓ recv_filter msg).
+  □ (□◊!↓send_filter msg → □◊!↓ any_recv_filter (m_destination msg) → ◊!↓ recv_filter msg).
 
 Definition retransmit_fair_network (mtr : mtrace) : Prop :=
   ∀ msg, retransmit_fair_network_delivery msg mtr.
 
 (* TODO: This should be generalised, and lifted to multiple roles *)
-Definition retransmit_terminating_role (ρ : retransmit_node_role) (tr : mtrace) : Prop :=
+Definition retransmit_terminating_role (ρ : retransmit_role) (tr : mtrace) : Prop :=
   (◊↓λ st _, ρ ∉ retransmit_live_roles st) tr ∨ ¬ infinite_trace tr.
 
-Definition retransmit_fair_scheduling_mtr (ρ : retransmit_node_role) : mtrace → Prop :=
+Definition retransmit_fair_scheduling_mtr (ρ : retransmit_role) : mtrace → Prop :=
   trace_always_eventually_implies_now
     (λ δ _, retransmit_role_enabled_model ρ δ)
-    (λ δ ℓ, ¬ retransmit_role_enabled_model ρ δ ∨
-              option_map label_role ℓ = Some (inl ρ)).
+    (λ δ (ℓ: option retransmit_label), ¬ retransmit_role_enabled_model ρ δ ∨
+              option_map fst ℓ = Some ρ).
 
 Definition retransmit_fair_scheduling (mtr : mtrace) : Prop :=
   ∀ ρ, retransmit_fair_scheduling_mtr ρ mtr.
@@ -170,9 +170,68 @@ Proof. apply trace_always_universal.
   by destruct mtr'; set_solver.
 Qed.
 
+Lemma B_always_live_infinite (mtr : mtrace) :
+  ¬ retransmit_terminating_role Brole mtr →
+  (□ (trace_now (λ s _, retransmit_role_enabled_model Brole s))) mtr.
+Proof.
+  intros Hnt. apply trace_alwaysI. intros mtr' Hsuff.
+  rewrite /trace_now /pred_at /retransmit_role_enabled_model.
+  have ? : Brole ∈ retransmit_live_roles (trfirst mtr'); last destruct mtr' =>//=.
+  apply NNP_P => Hin. apply Hnt.
+  rewrite /retransmit_terminating_role. left.
+  eapply (trace_eventually_suffix_of _ mtr') =>//. apply trace_eventually_intro.
+  by destruct mtr'.
+Qed.
+
+Lemma B_always_live_always_eventually_receive (mtr : mtrace) :
+  mtrace_fair mtr →
+  mtrace_valid mtr →
+  (□ (trace_now (λ s _, retransmit_role_enabled_model Brole s))) mtr →
+  (□◊!↓ any_recv_filter saB) mtr.
+Proof.
+  intros Hf Hval Hae. apply trace_alwaysI. intros mtr' Hsuff.
+  have Hfs': retransmit_fair_scheduling mtr'.
+  { by apply mtrace_fair_always, (trace_always_suffix_of _ _ _ Hsuff), trace_always_elim in Hf as [??]. }
+  rewrite /retransmit_fair_scheduling in Hfs'.
+  specialize (Hfs' Brole).
+  rewrite /retransmit_fair_scheduling_mtr in Hfs'.
+  rewrite /trace_always_eventually_implies_now in Hfs'.
+  rewrite /trace_always_eventually_implies in Hfs'.
+  have He: (↓ λ s _, retransmit_role_enabled_model Brole s) mtr'.
+  { apply trace_always_elim in Hfs'.
+    apply (trace_always_suffix_of _ _ _ Hsuff) in Hae.
+    by apply trace_always_elim in Hae. }
+  apply trace_always_elim in Hfs'.
+  rewrite trace_impliesI in Hfs'.
+  specialize (Hfs' He). clear He.
+  apply trace_eventuallyI in Hfs' as (mtr'' & Hsuff' & Hfs'').
+  apply (trace_eventually_suffix_of _ mtr'') =>//.
+  have Hsuff2: trace_suffix_of mtr'' mtr by eapply trace_suffix_of_trans.
+  have He: retransmit_role_enabled_model Brole (trfirst mtr'').
+  { apply (trace_always_suffix_of _ _ _ Hsuff2) in Hae.
+    eapply trace_always_elim in Hae. by destruct mtr''. }
+  destruct mtr'' as [|s [ρ α]]; destruct Hfs''=>//.
+  apply trace_eventually_intro=>//=.
+  rewrite /trace_now_label /pred_at /any_recv_filter /=.
+  apply (trace_always_suffix_of _ _ _ Hsuff2), trace_always_elim in Hval.
+  inversion Hval; simplify_eq; naive_solver.
+Qed.
+
+Lemma B_always_receives (mtr : mtrace) :
+  mtrace_fair mtr →
+  mtrace_valid mtr →
+  ¬ retransmit_terminating_role Brole mtr →
+  (□◊!↓ any_recv_filter saB) mtr.
+Proof.
+  intros Hf Hval Hnt.
+  apply B_always_live_infinite in Hnt.
+  apply B_always_live_always_eventually_receive in Hnt =>//.
+Qed.
+
+
 Lemma retransmit_fair_traces_eventually_A mtr :
   retransmit_fair_scheduling_mtr Arole mtr →
-  (◊ (↓ (λ _ ℓ, option_map label_role ℓ = Some $ inl Arole))) mtr.
+  (◊ (↓ (λ _ ℓ, option_map fst ℓ = Some $ Arole))) mtr.
 Proof.
   intros Hfair.
   pose proof (A_always_live mtr) as HA.
@@ -188,7 +247,7 @@ Qed.
 
 Lemma retransmit_fair_traces_eventually_mAB mtr :
   mtrace_valid mtr → retransmit_fair_scheduling_mtr Arole mtr →
-  (◊ ↓ send_filter mAB) mtr.
+  (◊ !↓ send_filter mAB) mtr.
 Proof.
   intros Hvalid Hfair.
   pose proof (retransmit_fair_traces_eventually_A mtr Hfair) as Htr.
@@ -199,15 +258,13 @@ Proof.
   destruct tr' as [s|s l tr']; [done|].
   apply trace_now_mono_strong.
   intros ???? HP; simplify_eq.
-  destruct l; [|done]. destruct r. simpl in *.
+  destruct l. destruct r=>//. simpl in *.
   simplify_eq. inversion Hvalid. inversion H1. by simplify_eq.
 Qed.
 
-(* Proof by the fact that A is always live, and will eventually be scheduled.
-   Needs fairness assumptions *)
 Lemma retransmit_fair_traces_always_eventually_mAB mtr :
   mtrace_valid mtr → retransmit_fair_scheduling_mtr Arole mtr →
-  (□ ◊ ↓ send_filter mAB) mtr.
+  (□ ◊ !↓ send_filter mAB) mtr.
 Proof.
   intros Hvalid Hfair. eapply trace_always_implies_always;
     [|apply trace_always_and; split; [apply Hvalid|apply Hfair]].
@@ -215,260 +272,52 @@ Proof.
   by apply retransmit_fair_traces_eventually_mAB.
 Qed.
 
-Lemma eventually_send_eventually_deliver mtr :
-  retransmit_fair_network mtr →
-  (□ ◊ ↓ send_filter mAB) mtr →
-  (◊ ↓ deliver_filter mAB) mtr.
-Proof.
-  intros Hfair_network Hsend.
-  pose proof (Hfair_network mAB). apply trace_always_elim in H.
-  rewrite trace_impliesI in H. apply H. done.
-Qed.
 
-(* If a message is delivered, the next state has a message in the buffer *)
-(* Proof by validity relation of the model *)
-Lemma deliver_next_buffer msg mtr :
-  mtrace_valid mtr →
-  (↓ deliver_filter msg) mtr →
-  (○ ↓ λ s _, ∃ bs, s.2 !!! (m_destination msg) = msg :: bs) mtr.
-Proof.
-  intros Hvalid%trace_always_elim Hdeliver.
-  destruct mtr; [done|].
-  exists mtr. split; [done|].
-  rewrite /trace_now /deliver_filter /pred_at in Hdeliver.
-  simpl in *. simplify_eq.
-  inversion Hvalid. simplify_eq.
-  destruct mtr.
-  - rewrite /trace_now /pred_at. simpl in *. simplify_eq.
-    exists (bs !!! m_destination msg).
-    simpl. by rewrite lookup_total_insert.
-  - rewrite /trace_now /pred_at. simpl in *. simplify_eq.
-    exists (bs !!! m_destination msg).
-    simpl. by rewrite lookup_total_insert.
-Qed.
-
-(* A scheduled B will succeed if there is something in the buffer *)
-(* Proof by validity relation of the model *)
-Lemma successful_deliver_received bs (mtr : mtrace) :
-  mtrace_valid mtr →
-  (↓ (λ s _, mAB :: bs `suffix_of` s.2 !!! (m_destination mAB))) mtr →
-  (↓ (λ _ l, option_map label_role l = Some (inl Brole))) mtr →
-  (○ ↓ (λ s _, s.1.1 = Received)) mtr.
-Proof.
-  intros Hvalid%trace_always_elim Hbs HB.
-  destruct mtr as [?|s l mtr]; [done|].
-  simpl in *. destruct l as [|]; [|done].
-  exists mtr. split; [done|].
-  rewrite /trace_now /pred_at in HB.
-  simpl in *. simplify_eq.
-  destruct r. simpl in *. simplify_eq.
-  inversion Hvalid; simplify_eq; [|]; last first.
-  { destruct mtr as [[]|[]]; simpl in *; simplify_eq; done. }
-    rewrite /trace_now /pred_at in Hbs. simpl in *.
-  rewrite H2 in Hbs. by apply suffix_cons_nil_inv in Hbs.
-Qed.
-
-Lemma B_enabled_not_received s :
-  retransmit_role_enabled_model Brole s ↔ s.1.1 ≠ Received.
-Proof.
-  rewrite /retransmit_role_enabled_model /retransmit_live_roles.
-  split.
-  - intros. destruct s as [[??]?]. simpl in *. intros ->. set_solver.
-  - intros. destruct s as [[??]?]. simpl in *.
-    apply elem_of_union. right. destruct r; set_solver.
-Qed.
-
-Lemma not_B_enabled_received s :
-  ¬ retransmit_role_enabled_model Brole s ↔ s.1.1 = Received.
-Proof.
-  rewrite /retransmit_role_enabled_model /retransmit_live_roles.
-  split.
-  - intros. destruct s as [[??]?]. simpl in *. destruct r; set_solver.
-  - intros. destruct s as [[??]?]. simpl in *. intros Helem.
-    simplify_eq. set_solver.
-Qed.
-
-Lemma received_or_eventually_B (mtr : mtrace) :
+Lemma B_terminates (mtr : mtrace) :
   mtrace_fair mtr →
-  (◊↓ λ s _, s.1.1 = Received) mtr ∨
-  (◊↓ λ _ l, option_map label_role l = Some $ inl Brole) mtr.
-Proof.
-  intros Hfair.
-  assert ((↓ λ s _, s.1.1 = Received) mtr ∨
-         ¬ (↓ λ s _, s.1.1 = Received) mtr).
-  { apply ExcludedMiddle. }
-  destruct H as [H|H].
-  { left. apply trace_eventually_intro. done. }
-  apply trace_notI in H. apply trace_now_not in H.
-  assert ((↓ (λ s _, retransmit_role_enabled_model Brole s)) mtr) as HB.
-  { revert H. apply trace_now_mono.
-    intros. by apply B_enabled_not_received. }
-  destruct Hfair as [Hfair _].
-  specialize (Hfair Brole).
-  apply trace_always_elim in Hfair.
-  rewrite trace_impliesI in Hfair.
-  apply Hfair in HB.
-  apply trace_eventually_or. revert HB.
-  apply trace_eventually_mono.
-  intros tr Htr.
-  apply trace_now_or in Htr.
-  destruct Htr as [Htr|Htr].
-  - left. revert Htr. apply trace_now_mono. intros.
-    by apply not_B_enabled_received.
-  - by right.
-Qed.
-
-(* Need to assume that trace is infinite *)
-Lemma retransmit_fair_trace_buffer_grow_next mtr bs :
-  infinite_trace mtr →
   mtrace_valid mtr →
-  (↓ λ s _, s.2 !!! (m_destination mAB) = bs) mtr →
-  (↓ λ _ l, option_map label_role l ≠ Some $ inl Brole) mtr →
-  (○ (↓ (λ s _, ∃ bs', bs `suffix_of` bs' ∧
-                       s.2 !!! m_destination mAB = bs'))) mtr.
-Proof.
-  intros Hinf Hvalid Hbs HBrole.
-  apply trace_always_elim in Hvalid.
-  destruct mtr.
-  { specialize (Hinf 1). by apply is_Some_None in Hinf. }
-  destruct mtr.
-  { specialize (Hinf 2). by apply is_Some_None in Hinf. }
-  destruct s as [[??]?].
-  rewrite /trace_now /pred_at.
-  rewrite /trace_now /pred_at in Hbs.
-  rewrite /trace_now /pred_at in HBrole.
-  simpl in *.
-  apply trace_next_intro.
-  inversion Hvalid; simplify_eq.
-  - exists (g !!! m_destination mAB). set_solver.
-  - exists (g !!! m_destination mAB). set_solver.
-  - exists (g !!! m_destination mAB). set_solver.
-  - destruct (decide (m_destination msg = saB)) as [->|Hneq].
-    + exists (msg :: g !!! m_destination mAB).
-      split; [by apply suffix_cons_r|].
-      simpl. rewrite lookup_total_insert. done.
-    + exists (g !!! m_destination mAB).
-      simpl. rewrite lookup_total_insert_ne; [|done].
-      set_solver.
-Qed.
-
-(* The buffers will only grow until B is scheduled *)
-(* Proof by validity relation of the model *)
-Lemma retransmit_fair_trace_buffer_grows mtr bs :
-  infinite_trace mtr →
-  mtrace_valid mtr →
-  mtrace_fair mtr →
-  (↓ λ s _, s.2 !!! (m_destination mAB) = bs) mtr →
-  ((◊trace_and
-     (↓ (λ s _, suffix bs (s.2 !!! (m_destination mAB))))
-     (↓ (λ _ l, option_map label_role l = Some $ inl Brole))) mtr) ∨
-  ((◊↓ λ s _, s.1.1 = Received) mtr).
-Proof.
-  intros Hinf Hvalid Hfair Hnow.
-  (* TODO: Need to assume not received instead *)
-  pose proof (received_or_eventually_B mtr Hfair) as [Hreceived|HB].
-  { right. done. }
-  left.
-  revert bs Hnow.
-  apply trace_eventually_until in HB.
-  induction HB; intros bs Hnow.
-  { eapply trace_eventually_mono; [apply trace_now_and|].
-    apply trace_eventually_intro.
-    pose proof (trace_now_split _ _ _ Hnow H) as Hnow'.
-    revert Hnow'. apply trace_now_mono.
-    intros s l [H1 H2]. split; [|done]. set_solver. }
-  apply trace_eventually_cons.
-  assert (∃ bs', bs `suffix_of` bs' ∧
-             (↓ (λ s _ , s.2 !!! m_destination mAB = bs'))
-               tr) as [bs' [Hbs' Hnow']].
-  { assert ((↓ (λ s _, ∃ bs', bs `suffix_of` bs' ∧ s.2 !!! m_destination mAB = bs'))
-               tr) as H'; last first.
-    { apply trace_now_exists in H' as [bs' H'].
-      exists bs'.
-      rewrite /trace_now /pred_at.
-      rewrite /trace_now /pred_at in H'.
-      destruct tr; simpl in *; done. }
-    eapply trace_next_elim.
-    by apply retransmit_fair_trace_buffer_grow_next. }
-    eapply trace_eventually_mono; last first.
-  { assert (mtrace_valid tr) as Hvalid' by by eapply trace_always_cons.
-    apply mtrace_fair_always in Hfair.
-    assert (mtrace_fair tr) as Hfair'.
-    { apply mtrace_fair_always. by eapply trace_always_cons. }
-    assert (infinite_trace tr) as Hinf'.
-    { by eapply infinite_cons. }
-    apply (IHHB Hinf' Hvalid' Hfair' bs').
-    done. }
-  intros tr' H'. apply trace_andI. apply trace_andI in H'.
-  destruct H' as [H1 H2].
-  split; [|done].
-  revert H1. apply trace_now_mono.
-  intros ???. by etransitivity.
-Qed.
-
-Lemma eventually_deliver_eventually_received mtr :
-  infinite_trace mtr → mtrace_valid mtr → mtrace_fair mtr →
-  (◊ ↓ deliver_filter mAB) mtr →
-  (◊ ↓ λ s _, s.1.1 = Received) mtr.
-Proof.
-  intros Hinf Hvalid Hfair Hdeliver.
-  eapply trace_eventually_mono_strong in Hdeliver; last first.
-  { intros tr' Hsuffix. apply deliver_next_buffer. by eapply trace_always_suffix_of. }
-  apply trace_eventually_next in Hdeliver.
-  apply trace_eventually_idemp.
-  revert Hdeliver.
-  apply trace_eventually_mono_strong.
-  intros mtr' Hsuffix Hdeliver.
-  apply trace_now_exists in Hdeliver as [bs Hdeliver].
-  assert (infinite_trace mtr') as Hinf'.
-  { destruct Hsuffix as [n Hn].
-    eapply (infinite_trace_after n) in Hinf.
-    by rewrite Hn in Hinf. }
-  assert (mtrace_valid mtr') as Hvalid'.
-  { by eapply trace_always_suffix_of. }
-  assert (mtrace_fair mtr') as Hfair'.
-  { apply mtrace_fair_always in Hfair.
-    apply mtrace_fair_always. by eapply trace_always_suffix_of. }
-  pose proof (retransmit_fair_trace_buffer_grows _ (mAB :: bs) Hinf' Hvalid' Hfair' Hdeliver) as [H'|H']; last first.
-  { done. }
-  apply trace_eventually_next.
-  revert H'.
-  apply trace_eventually_mono_strong.
-  intros mtr'' Hsuffix' [Hmtr1'' Hmtr2'']%trace_andI.
-  assert (mtrace_valid mtr'') by by eapply trace_always_suffix_of.
-  by eapply successful_deliver_received.
-Qed.
-
-(* Any fair trace terminates on role B *)
-Lemma retransmit_fair_traces_terminate mtr :
-  mtrace_valid mtr → mtrace_fair mtr →
   retransmit_terminating_role Brole mtr.
 Proof.
-  intros Hvalid [Hfair1 Hfair2].
-  assert (infinite_trace mtr ∨ ¬ infinite_trace mtr) as [Hafter|Hafter];
-    [by apply ExcludedMiddle| |]; last first.
-  { by right. }
-  left.
-  pose proof (retransmit_fair_traces_always_eventually_mAB mtr Hvalid (Hfair1 _)).
-  apply (eventually_send_eventually_deliver _ Hfair2) in H.
-  apply (eventually_deliver_eventually_received) in H; [|done..].
-  revert H. apply trace_eventually_mono.
-  intros tr. apply trace_now_mono. intros [[]] _ Hreceived.
-  rewrite /retransmit_live_roles. simpl in *.
-  simplify_eq. set_solver.
+  intros Hf Hval. apply NNP_P. intros Hnt.
+  have Haer := Hnt.
+  apply B_always_receives in Haer =>//.
+  have Haes: (□ ◊ !↓ send_filter mAB) mtr.
+  { apply retransmit_fair_traces_always_eventually_mAB =>//. destruct Hf =>//. }
+  have Har: (◊ !↓ recv_filter mAB) mtr.
+  { destruct Hf as [Hsf Hnf].
+    specialize (Hnf mAB).
+    apply trace_always_elim in Hnf.
+    rewrite !trace_impliesI in Hnf.
+    naive_solver. }
+  apply trace_eventuallyI in Har as (mtr' & Hsuff & Hr).
+  destruct mtr' as [| s [ρ α] mtr'']; first naive_solver.
+
+  apply Hnt.
+  left. apply trace_eventuallyI. exists mtr''. split.
+  { eapply trace_suffix_of_trans=>//. exists 1. done. }
+
+  apply (trace_always_suffix_of _ _ _ Hsuff), trace_always_elim in Hval.
+  have ? : Brole ∉ retransmit_live_roles (trfirst mtr'').
+  { rewrite /trace_now_label /pred_at /recv_filter /= in Hr.
+    inversion Hval; simplify_eq; try set_solver. }
+  rewrite /trace_now /pred_at /=. destruct mtr''=>//.
 Qed.
 
-Definition retransmit_fair_model : FairModel.
+
+Definition retransmit_lts : Lts (retransmit_role * option (action aneris_lang)).
 Proof.
   refine({|
-            fmstate := retransmit_state;
-            fmrole := retransmit_node_role;
-            fmaction := retransmit_node_action;
-            fmconfig := retransmit_network_label;
-            fmtrans := retransmit_trans;
-            fmfairness := retransmit_fair_network;
-            live_roles := retransmit_live_roles;
-            fm_live_spec := retransmit_live_spec_holds;
-            fm_fl _ := 10;
+            lts_state := retransmit_state;
+            lts_trans := retransmit_trans;
+          |}).
+Defined.
+Definition retransmit_fair_model : UserModel aneris_lang.
+Proof.
+  refine({|
+            usr_role := retransmit_role;
+            usr_lts := retransmit_lts;
+            usr_live_roles := retransmit_live_roles;
+            usr_live_spec := retransmit_live_spec_holds;
+            usr_fl _ := 10;
           |}).
 Defined.
